informal proof of main search theorem

Lean4Axiomatic/Natural/Core.lean
@@ -8,7 +8,7 @@ Closely follows the [Peano axioms](https://en.wikipedia.org/wiki/Peano_axioms).
 
 namespace Lean4Axiomatic.Natural
 
-open Relation.Equivalence (EqvOp ite_subst_cond)
+open Relation.Equivalence (EqvOp)
 
 /-!
 ## Axioms
@@ -354,110 +354,5 @@ theorem step_neqv {n : ℕ} : step n ≄ n := by
     apply ih
     show step n ≃ n
     exact AA.inject ‹step (step n) ≃ step n›
-
-variable [Induction.{1} ℕ]
-
-/-- TODO -/
-def find_first_up_to
-    (P : ℕ → Prop) [DecidablePred P] (limit : ℕ) : Option ℕ
-    := by
-  apply ind_on limit (motive := λ _ => Option ℕ)
-  case zero =>
-    exact if P 0 then some 0 else none
-  case step =>
-    intro (n : ℕ) (rOpt : Option ℕ)
-    show Option ℕ
-    exact if rOpt.isNone && P (step n) then some (step n) else rOpt
-
-/-- TODO -/
-theorem find_first_up_to_false
-    {m : ℕ} : let P := λ _ => False; find_first_up_to P m ≃ none
-    := by
-  intro (P : ℕ → Prop)
-  show find_first_up_to P m ≃ none
-
-  let z := if P 0 then some 0 else none
-  let s := λ (n : ℕ) (rOpt : Option ℕ) =>
-    if rOpt.isNone && P (step n) then some (step n) else rOpt
-
-  apply ind_on m (motive := λ x => find_first_up_to P x ≃ none)
-  case zero =>
-    show find_first_up_to P 0 ≃ none
-    calc
-      _ = find_first_up_to P 0           := rfl
-      _ = ind_on 0 z s                   := rfl
-      _ ≃ z                              := ind_zero
-      _ = if P 0 then some 0 else none   := rfl
-      _ = if False then some 0 else none := rfl
-      _ = none                           := rfl
-  case step =>
-    intro (k : ℕ) (ih : find_first_up_to P k ≃ none)
-    show find_first_up_to P (step k) ≃ none
-
-    let rOpt := ind_on k z s
-    let rin := rOpt.isNone
-    let ssk := some (step k)
-    calc
-      _ = find_first_up_to P (step k)             := rfl
-      _ = ind_on (step k) z s                     := rfl
-      _ ≃ s k (ind_on k z s)                      := ind_step
-      _ = s k rOpt                                := rfl
-      _ = if rin && P (step k) then ssk else rOpt := rfl
-      _ = if rin && False then ssk else rOpt      := rfl
-      _ = if rin && false then ssk else rOpt      := rfl
-      _ = if false then ssk else rOpt             := by rw [Bool.and_false]
-      _ = rOpt                                    := rfl
-      _ = ind_on k z s                            := rfl
-      _ = find_first_up_to P k                    := rfl
-      _ ≃ none                                    := ih
-
-/-- TODO -/
-theorem find_first_up_to_true
-    {m : ℕ} : let P := λ _ => True; find_first_up_to P m ≃ some 0
-    := by
-  intro (P : ℕ → Prop)
-  show find_first_up_to P m ≃ some 0
-
-  let z := if P 0 then some 0 else none
-  let s := λ (n : ℕ) (rOpt : Option ℕ) =>
-    if rOpt.isNone && P (step n) then some (step n) else rOpt
-
-  apply ind_on m (motive := λ x => find_first_up_to P x ≃ some 0)
-  case zero =>
-    show find_first_up_to P 0 ≃ some 0
-    calc
-      _ = find_first_up_to P 0          := rfl
-      _ = ind_on 0 z s                  := rfl
-      _ ≃ z                             := ind_zero
-      _ = if P 0 then some 0 else none  := rfl
-      _ = if True then some 0 else none := rfl
-      _ = some 0                        := rfl
-  case step =>
-    intro (k : ℕ)
-    let rOpt := find_first_up_to P k
-    intro (ih : rOpt ≃ some 0)
-    show find_first_up_to P (step k) ≃ some 0
-
-    let psk := P (step k)
-    let ssk := some (step k)
-    have eh : (rOpt.isNone && psk) ≃ ((some 0).isNone && psk) := calc
-      _ ≃ (rOpt.isNone && psk) := Rel.refl
-      _ ≃ ((some 0).isNone && psk) := by srw [ih]
-    calc
-      _ = find_first_up_to P (step k)                  := rfl
-      _ = ind_on (step k) z s                          := rfl
-      _ ≃ s k (ind_on k z s)                           := ind_step
-      _ = s k (find_first_up_to P k)                   := rfl
-      _ = s k rOpt                                     := rfl
-      _ = if rOpt.isNone && psk then ssk else rOpt     := rfl
-      _ ≃ if (some 0).isNone && psk then ssk else rOpt := ite_subst_cond eh
-      _ = if false && psk then ssk else rOpt           := rfl
-      _ = if false then ssk else rOpt                  := rfl
-      _ = rOpt                                         := rfl
-      _ ≃ some 0                                       := ih
-
--- prove:
--- find_first_up_to (· ≃ m) m ≡ .some m
--- find_first_up_to P m ≡ Option.when(k ≤ m)(k), where P has first at k
 
 end Lean4Axiomatic.Natural
